



Exercise 1.1 Make sure you understand how to derive formula (1.7) using function $\varphi(t) = f(x + td)$.

▼ Solution

Similarly, we can prove the *mean value theorem*: for a differentiable f and any x, d there exists $z \in [x, x + d]$ such that

$$f(x + d) = f(x) + \langle \nabla f(z), d \rangle. \quad (1.7)$$

Mean value theorem.

For differentiable f and $(\forall x, d)(\exists z \in [x, x + d])$ s.t.

$$f(x + d) = f(x) + \langle \nabla f(z), d \rangle$$

Proof.

Consider the function $\varphi(t) = f(x + td)$:

φ is differentiable. We can find its derivative using the chain rule:

$$\varphi'(t) = f'(x + td)d = \langle \nabla f(x + td), d \rangle$$

Therefore, we can apply the mean value theorem to φ at $[0, 1]$:

$$\varphi(1) - \varphi(0) = \varphi'(t_0), \text{ for some } t_0 \in (0, 1).$$

By setting $z = x + t_0d$ and plugging f back, we get:

$$f(x + d) = f(x) + \langle \nabla f(z), d \rangle, \text{ for } z \in (x, x + d)$$



Exercise 1.2 Let $f(x) = \frac{1}{2}\|Ax - b\|^2$ for $A \in \mathbb{R}^{m \times n}$ and $b \in \mathbb{R}^m$. Compute the gradient in two ways: using the definition (1.5) and using the chain rule. ■

▼ **Solution**

Using the definition:

A function $f : \mathbb{R}^n \rightarrow \mathbb{R}$ is called differentiable at $x \in \mathbb{R}^n$ if there is $u \in \mathbb{R}^n$ such that for all $d \in \mathbb{R}^n$ we have

$$f(x + d) = f(x) + \langle u, d \rangle + o(\|d\|)$$

Let's consider the difference:

$$\begin{aligned} & f(x + d) - f(x) \\ &= \frac{1}{2}(\|A(x + d) - b\|^2 - \|Ax - b\|^2) \\ &= \frac{1}{2}(\|Ax - b + Ad\|^2 - \|Ax - b\|^2) \\ &= \frac{1}{2}(\|Ax - b\|^2 + 2\langle Ax - b, Ad \rangle + \|Ad\|^2 - \|Ax - b\|^2) \\ &= \frac{1}{2}(2\langle Ax - b, Ad \rangle + \|Ad\|^2) \\ &= \frac{1}{2}(2\langle A^\top(Ax - b), d \rangle + \|Ad\|) \\ &= \langle A^\top(Ax - b), d \rangle + \frac{\|Ad\|}{2} \end{aligned}$$

$$\Rightarrow u = \nabla f(x) = A^\top(Ax - b)$$

Using Chain Rule:

Let $h(x) = \frac{1}{2}\|x\|^2$, $g(x) = Ax - b$, then $f(x) = h(g(x))$

By the Chain Rule have:

$$\nabla f(x) = g'(x)^\top \nabla h(g(x))$$

As $g(x)$ is an affine function: $g'(x) = A$

Since $h(x) = \frac{1}{2} \sum x_j^2$, $\nabla h(x) = x$

$$\nabla f(x) = A^\top(Ax - b)$$



Exercise 1.3 Find the gradient and the Hessian of $f(x) = \frac{1}{2}\langle Qx, x \rangle - \langle b, x \rangle + c$, where $x, b \in \mathbb{R}^n$, $Q \in \mathbb{R}^{n \times n}$, and $c \in \mathbb{R}$. ■

▼ **Solution**

Just like in the previous task:

$$f(x + d) = f(x) + \langle u, d \rangle + o(\|d\|)$$

Considering the difference:

$$\begin{aligned} f(x + d) - f(x) &= \frac{1}{2}((x + d)^\top Q(x + d) - x^\top Qx) - b^\top d \\ &= \frac{1}{2}(x^\top Qd + d^\top Qx + d^\top Qd) - b^\top d \\ &= \frac{1}{2}(\langle Q^\top x, d \rangle + \langle Qx, d \rangle) - \langle b, d \rangle + \frac{1}{2}\langle Qd, d \rangle \\ &\Rightarrow u = \nabla f(x) = Qx - b \end{aligned}$$

Hessian:

$$\nabla^2 f(x) = [\nabla f(x)]' = Q$$



Exercise 1.4 Make sure you understand what equation (1.10) means and why that derivation is correct. 1.10

▼ **Solution**

1. (Gradients define the direction of the local fastest increase of f :)

$$\frac{\nabla f(x)}{\|\nabla f(x)\|} = \operatorname{argmax}_{\|d\|=1} \lim_{t \rightarrow 0} \frac{f(x + td) - f(x)}{t} = \operatorname{argmax}_{\|d\|=1} \langle \nabla f(x), d \rangle.$$

This follows directly from the Cauchy-Schwarz inequality.

By **Cauchy–Bunyakovsky–Schwarz** inequality $|\langle \nabla f(x), d \rangle| \leq \|\nabla f(x)\| \|d\|$

Since it is sufficient to only choose direction from vectors of $\|d\| = 1$, we can maximize $\langle \nabla f(x), d \rangle$ by setting $d = \frac{\nabla f(x)}{\|\nabla f(x)\|}$.



Exercise 1.5 When is the function defined in Exercise 1.3 (i) convex; (ii) strongly convex? 1.3

▼ **Solution**

Exercise 1.3 Find the gradient and the Hessian of $f(x) = \frac{1}{2} \langle Qx, x \rangle - \langle b, x \rangle + c$, where $x, b \in \mathbb{R}^n$, $Q \in \mathbb{R}^{n \times n}$, and $c \in \mathbb{R}$.

(i) $(Q + Q^\top)$ is positive semidefinite

(ii) $(Q + Q^\top) \succeq \mu I$ for some positive μ



Exercise 1.6 Prove equivalence in (ii) in Lemma 1.2. ■

▼ Solution

- f is μ -strongly convex if and only if

$$f(y) \geq f(x) + \langle \nabla f(x), y - x \rangle + \frac{\mu}{2} \|y - x\|^2 \quad \text{for all } x, y. \quad (1.15)$$

By definition of strong convexity:

μ -strongly convex if

$$\lambda f(x) + (1 - \lambda)f(y) \geq f(\lambda x + (1 - \lambda)y) + \frac{\mu\lambda(1 - \lambda)}{2} \|x - y\|^2 \quad \forall x, y \quad \forall \lambda \in [0, 1] \quad (1.13)$$

(\Rightarrow) Assume that function is strongly convex and

$$f(x) - f(y) \geq \frac{f(y + \lambda(x - y)) - f(y)}{\lambda} + \frac{\mu(1 - \lambda)}{2} \|x - y\|^2$$

Since $f(x)$ is differentiable, letting $\lambda \rightarrow 0$, got

$$f(x) - f(y) \geq \langle \nabla f(y), x - y \rangle + \frac{\mu}{2} \|x - y\|^2$$

Conversely (\Leftarrow)

Take $z = \lambda x + (1 - \lambda)y$

$$f(x) \geq f(z) + \langle \nabla f(z), x - z \rangle + \frac{\mu}{2} \|x - z\|^2$$

$$f(y) \geq f(z) + \langle \nabla f(z), y - z \rangle + \frac{\mu}{2} \|y - z\|^2$$

Multiplying the first inequality by λ and the second one by $1 - \lambda$ and adding them up leads to the definition of μ -strongly convex functions. To see that:

$$\begin{aligned} x - z &= x - \lambda x - (1 - \lambda)y = (1 - \lambda)(x - y) \\ y - z &= y - \lambda x - (1 - \lambda)y = \lambda(y - x) \end{aligned}$$

yielding $\lambda(x - z) + (1 - \lambda)(y - z) = 0$.



Exercise 1.7 One may expect that in Lemma 1.3, strict convexity is equivalent to $\nabla^2 f(x) \succ 0$. Show that this is not true. ■

▼ **Solution**

Consider $f(x) = x^4$ It is strictly convex:

$$\begin{aligned} & \forall x, y \in \mathbb{R} \\ & (1 - \alpha)x^4 + \alpha y^4 > ((1 - \alpha)x + \alpha y)^4 \\ & ((1 - \alpha)x + \alpha y)^4 = (((1 - \alpha)x + \alpha y)^2)^2 \end{aligned}$$

Since $g(x) = x^2$ is strictly convex have

$$(((1 - \alpha)x + \alpha y)^2)^2 < ((1 - \alpha)x^2 + \alpha y^2)^2 < (1 - \alpha)x^4 + \alpha y^4$$



Exercise 1.8 Prove Lemma 1.4.

Lemma 1.4 Let $f : \mathbb{R}^n \rightarrow \mathbb{R}$. The following holds:

- (i) If f is convex, then every local minimum is a global one and the set of minima is convex.
- (ii) If f is strictly convex, then it has at most one minimum.
- (iii) If f is strongly convex, then minimum always exists.

▼ **Solution**

(i) Proof. By contradiction, let x_1, x_2 be local minima such that $f(x_1) < f(x_2)$.

Take some neighborhood $B(x_2, \alpha_2), \forall y \in B(x_2, \alpha_2) : f(y) \geq f(x_2)$. Such neighborhood always exist by definition of local minimum. But then, for all small enough $t \in (0, \alpha_2]$:

$$f((1-t)x_2 + tx_1) \geq f(x_2) > (1-t)f(x_2) + tf(x_1)$$

Which is a contradiction of f being convex.

Now let us prove that the set of minima is convex:

by contradiction, let us assume that x, y - global minima, but $z = (1-t)x + ty, t \in (0, 1)$ isn't one.

By definition of convexity, we have:

$$(1-t)f(x) + tf(y) = f(x) \geq f(z)$$

However, we have previously stated that $f(z) > f(x)$. Therefore, we get a contradiction, and thus the set of minima is convex.

(ii) Proof. Suppose there are more than one minimum. Take two arbitrary points x_1, x_2 that minimize the function f . By (i) $f(x_1) = f(x_2)$, as strict convexity implies convexity.

We can consider three possible cases:

1. f attains value greater than $f(x_1), f(x_2)$ on interval $[x_1, x_2]$.
This would clearly contradict definition of strict convexity.
2. f attains the same values as $f(x_1), f(x_2)$ on interval $[x_1, x_2]$.
This would also contradict strict inequality in definition of strict convexity.

3. f attains values smaller $f(x_1), f(x_2)$ on interval $[x_1, x_2]$. But then this contradicts part (i).

(iii) Proof.

By definition of strong convexity (by taking $y = 0$)

$$(1 - \lambda)f(x) + \lambda f(0) \geq f((1 - \lambda)x) + \frac{\mu\lambda(1 - \lambda)}{2} \|x\|^2, \quad \forall x, \forall \lambda \in [0, 1]$$

Setting $\lambda = \frac{1}{2}$ we get

$$f(x) \geq 2f\left(\frac{x}{2}\right) - f(0) + \frac{\mu}{4} \|x\|^2$$

Since $f(x) \geq 2f\left(\frac{x}{2}\right) - f(0)$ by convexity, as $\|x\| \rightarrow \infty$ whole RHS goes to infinity, thus $f(x) \rightarrow \infty$. Then $(\forall M \in \mathbb{R})(\exists k \in \mathbb{R}_+)(\forall x : \|x\| \geq k)\{f(x) \geq M\}$.

Therefore, for arbitrary M , we can find such k so that the minima has to belong to a closed ball $B(0, k)$.

Then, by theorem of Weierstrass a continuous function on closed and bounded set attains its minimum and maximum \Rightarrow minimum always exist.



Exercise 2.1 Show that the update in (2.3) is indeed equivalent to the GD update. ■

▼ Solution

2. Minimizing f is hard, so let's minimize its Taylor's approximation around x_k . Consider the first-order approximation

$$f(x) \approx f(x_k) + \langle \nabla f(x_k), x - x_k \rangle.$$

This approximation is linear over x , so minimizing it doesn't make much sense — we always obtain $-\infty$. To prevent this, we can add some regularization and thus, we define x_{k+1} as

$$x_{k+1} = \operatorname{argmin}_x \left\{ f(x_k) + \langle \nabla f(x_k), x - x_k \rangle + \frac{1}{2a_k} \|x - x_k\|^2 \right\}. \quad (2.3)$$

It is easy to check that this will lead to GD as in (2.2).

Dropping the terms not dependent on x , we have:

Let us consider function

$$g(x) = f(x_k) + \langle \nabla f(x_k), x - x_k \rangle + \frac{1}{2a_k} \|x - x_k\|^2$$

It's gradient is:

$$\nabla g(x) = \nabla f(x_k) + \frac{1}{a_k} (x - x_k)$$

And Hessian is:

$$\nabla^2 g(x) = \frac{1}{a_k} I$$

Since $\nabla^2 g(x) \succeq \frac{1}{a_k} \cdot g(x)$ is strongly convex and, thus, have one local minimum, which is also global. By optimality condition $\nabla g(x) = 0$.

$$\begin{aligned} 0 &= a_k \nabla f(x_k) + x - x_k \\ x &= x_k - a_k \nabla f(x_k) \end{aligned}$$

Then call this minimizer as $x_{k+1} := x$ Which gives GD iteration

$$x_{k+1} = x_k - \alpha_k \nabla f(x_k)$$



Exercise 2.2 Show that $\alpha = \frac{1}{L}$ is indeed the maximum of $\alpha(2 - \alpha L)$. ■

▼ **Solution**

$$\frac{d}{d\alpha}(\alpha(2 - \alpha L)) = 2 - \alpha L - \alpha L = 0 \Rightarrow \alpha = \frac{1}{L}$$



Exercise 2.3 Prove that f in (2.7) is convex if and only if $Q \succcurlyeq 0$. ■

▼ **Solution**

$$f(x) = \frac{1}{2} \langle Qx, x \rangle - \langle b, x \rangle, \quad (2.7)$$

$$\nabla^2 f(x) = \frac{1}{2}(Q + Q^\top),$$

$f(x)$ is convex if and only if $\nabla^2 f(x) \succeq 0$.

Under the implicit assumption that Q is symmetric, this indeed becomes equivalent to $Q \succeq 0$.



Exercise 2.4 Prove that f in (2.7) is L -smooth, with $L = \|Q\| = \lambda_{\max}(Q)$. ■

▼ **Solution**

$$f(x) = \frac{1}{2} \langle Qx, x \rangle - \langle b, x \rangle, \quad (2.7)$$

$$\nabla^2 f(x) = \frac{1}{2} (Q + Q^\top),$$

$f(x)$ is L -smooth if and only if $\nabla^2 f(x) \preceq LI$.

Under the implicit assumption that Q is symmetric, this becomes equivalent to $\lambda_{\max}(Q) \leq L$. Therefore, statement proven.



Exercise 2.6 Prove that $1 - t \leq e^{-t}$ using only convexity arguments (one line proof). ■

▼ **Solution**

$f(t) = e^{-t}$ is differentiable and convex; let us use an alternative definition of convexity for a differentiable function, i.e., that

$$f(t) \geq f(0) + tf'(0):$$

$$e^{-t} \geq e^0 - e^0 t = 1 - t$$